lean-fx-2/LeanFX2/Algo/Soundness.lean
@@ -416,7 +416,7 @@ theorem Term.headStep?_sound
   | modIntro _ => nomatch firedEq
   | subsume _ => nomatch firedEq
   | universeCode _ _ _ _ => nomatch firedEq
-  | cumulUp _ _ _ _ _ _ _ _ _ => nomatch firedEq
+  | cumulUp _ _ _ _ _ _ => nomatch firedEq
   | equivReflId _ => nomatch firedEq
   | funextRefl _ _ _ => nomatch firedEq
   | equivReflIdAtId _ _ _ _ => nomatch firedEq
